This is a basic example of the addition of 2 power series $f(x)$ and $g(x)$.

Let:
$F(x) = \sum_{n=0}^\infty a_{n}n(n+1)x^n$, and $g(x) = \sum_{r=0}^\infty 2a_{n}(n+1)x^n$.

The addition of $f(x) + g(x)$ is very intuitive, simply add the coefficients as the power term in both is equivalent.

$$
f(x) + g(x) = \sum_{n=0}^\infty [a_{n}n(n+1) + 2a_{n}(n+1)] x^n
$$
_this can be simplified but idgaf_

---

Now let:
$F(x) = (1+x^{2})$ and $g(x) = \sum_{n=0}^\infty a_{n}x^n$.

The multiplication of these two functions is also intuitive. $$
f(x)g(x) = \sum_{n=0}^\infty a_{n}(1+x^{2})x^n
$$
This simplifies into:
$$
\sum_{n=0}^\infty a_{n}x^n + \sum_{n=0}^\infty a_{n}x^{n+2}
$$
---

