To solve a normal ODE, we find the CF, we take the equation with RHS = 0, and make a guess $y=e^{mx}$, and solve the auxiliary equation, then our CF will take some form of $y = c_{1}e^{m_{1}x} + c_{2}e^{m_{2}x}$, depending on what kind of ODE we were given.

Then for the PI, we look at the RHS = $f(x)$, taking a guess for y based on the form of $f(x)$. Then we can use the [[Principle of superposition]] to build a linear combination of solutions.

Now we will extend these ideas to account of ODES with variable coefficients:
$$
a(x)y'' + b(x)y' + c(x) = 0
$$
