<H1>Line Integrals</H1>
### [Example 4.8]
Show that $$
\underline{F}=(6x-2e^{2x}y^{2})\underline{i} + 2ye^{2x}\underline{j}+\cos z\underline{k}
$$
is conservative and evaluate $\int _{c}\underline{F}\cdot \, d\underline{r}$ at $$\underline{r}(t) = t\underline{i}+(t-1)(t-2)\underline{j}+\frac{\pi}{2}t^{3}\underline{k}, \,\,0\leq t\leq 1

$$
Note for F to be conservative then its curl will be 0.

$$
curl(F)=\begin{vmatrix}
\underline{i} & \underline{j} & \underline{k} \\
\frac{\partial}{\partial x} & \frac{\partial}{\partial y} & \frac{\partial}{\partial z} \\
6x-2e^{2x}y & 2ye^{2x} & \cos z
\end{vmatrix}
$$

This is $\equiv$ to $\underline{0}$, Therefore F is conservative.

So, $\int _{c} \underline{F}\cdot \, dc=\phi(\underline{r}_{1})-\phi(\underline{r}_{0})$ where $F=grad(\phi)$:

$$
\begin{gather}
grad\phi=\underline{F}\\\implies \frac{\partial f}{\partial x} =6x-2e^{2x}y^x
\\\frac{\partial f}{\partial y}=-2ye^{2}x
\\ \frac{\partial z}{\partial z}=\cos z
\end{gather}

$$

From $\frac{\partial f}{\partial x}$, we get:
$$
\phi=3x^{2}-e^{2x}y^{2}+F_{1}(y,z)
$$
For some $F_{1}$

Subbing $\frac{\partial}{\partial x}$ into $\frac{\partial}{\partial y}$ we get:
$$
-2e^{-2x}y+\frac{\partial}{\partial y}=-2ye^{2x}
$$
So,
$$
\frac{\partial}{\partial y} = 0 \,\,\,,\,\,\,F_{1}(y,z)=F_{2}(z)
$$
$$
\phi=3x^{2}=e^{2x}y^{2}+F_{2}(z)
$$
Subbing this into $\frac{\partial}{\partial z}$ we get:
$$
\frac{\partial}{\partial z}=\cos z
$$
$$
F_{2}(zz)=\sin z+c
$$
For some constant C, So:
$$
\phi=3x^{2}-e^{3x}y^{2}+\sin z+c
$$
Then:
$$
\underline{r}(t)=(t,(t-1)(t-2),\frac{\pi}{2}t^{3})\,\,\,\, 0\leq t\leq 1
$$
$$
t=0\implies x=0\,\,y=0\,\,z=0\,\,\implies \phi|_{t=1}=3+0+1+c=4+c
$$
Therefore,
$$
\int _{c}f\cdot  \, dc=\phi(\underline{r_{1}})+\phi(\underline{r_{2}})
$$
$Q\mathbf{E}D$

